commit

AP/Util/Set.lean
@@ -1,3 +1,4 @@
+import AP.Util.Option
 import AP.Util.Fintype
 
 noncomputable
@@ -9,30 +10,24 @@ def Set.Finite.toFintype {α : Type*}
 
 namespace Set
 
-def erase {α : Type*} (x : α) (s : Set α) := s \ {x}
+variable {α β : Type*} {s s' : Set α}
+
+def erase (x : α) (s : Set α) := s \ {x}
 
 @[simp]
-theorem mem_erase {α : Type*} {z x : α} (s : Set α) :
-z ∈ s.erase x ↔ z ≠ x ∧ z ∈ s := by
+theorem mem_erase {z x : α} : z ∈ s.erase x ↔ z ≠ x ∧ z ∈ s := by
   unfold erase; aesop
 
-theorem erase_eq_of_not_mem {α : Type*} {x : α} {s : Set α}
-(h : x ∉ s) : s.erase x = s := by simpa [erase]
+theorem erase_eq_of_not_mem {x : α} (h : x ∉ s) : s.erase x = s := by
+  simpa [erase]
 
-theorem insert_erase_eq_of_mem {α : Type*} {x : α} {s : Set α}
-(h : x ∈ s) : insert x (s.erase x) = s := by
+theorem insert_erase_eq_of_mem {x : α} (h : x ∈ s) : insert x (s.erase x) = s := by
   ext z; simp; apply Iff.intro <;> intro h₁
   rcases h₁ with rfl | ⟨h₁, h₂⟩ <;> assumption
   simp [h₁]; apply eq_or_ne
 
-theorem ne_none_of_eq_some {α : Type*} {m : Option α} {x : α}
-(h : m = some x) : m ≠ none := by simp [h]
-
-def List.snoc {α : Type*} (xs : List α) (x : α) := xs ++ [x]
-
 @[simp]
-theorem finite_erase_iff {α : Type*} {x : α} {s : Set α} :
-(s.erase x).Finite ↔ s.Finite := by
+theorem finite_erase_iff {x : α} : (s.erase x).Finite ↔ s.Finite := by
   by_cases hx : x ∈ s
   case neg => simp [erase_eq_of_not_mem hx]
   symm; apply Iff.intro Finite.diff; intro h
@@ -43,44 +38,63 @@ theorem finite_erase_iff {α : Type*} {x : α} {s : Set α} :
   apply Finite.insert; exact h
 
 @[simp]
-theorem infinite_erase_iff {α : Type*} {x : α} {s : Set α} :
-(s.erase x).Infinite ↔ s.Infinite := by simp [Set.Infinite]
+theorem infinite_erase_iff {x : α} : (s.erase x).Infinite ↔ s.Infinite := by
+  simp [Set.Infinite]
 
-theorem diff_upair {α : Type*} (x y : α) (s : Set α) :
-s \ {x, y} = (s \ {x}) \ {y} := by ext z; simp; tauto
+theorem diff_upair (x y : α) (s : Set α) : s \ {x, y} = (s \ {x}) \ {y} := by
+  ext z; simp; tauto
 
 @[simp]
-theorem univ_ne_univ_diff_insert {α : Type*} {x : α} {s : Set α} :
-univ ≠ univ \ (insert x s) := by
+theorem univ_ne_univ_diff_insert {x : α} : univ ≠ univ \ (insert x s) := by
   simp [Set.ext_iff]; use x; simp
 
 @[simp]
-theorem univ_ne_univ_diff_singleton {α : Type*} {x : α} :
-univ ≠ univ \ {x} := by simp [Set.ext_iff]
+theorem univ_ne_univ_diff_singleton {x : α} : univ ≠ univ \ {x} := by
+  simp [Set.ext_iff]
 
 @[simp]
-theorem univ_ne_erase {α : Type*} {x : α} :
-univ ≠ univ.erase x := by simp [erase]
+theorem univ_ne_erase {α : Type*} {x : α} : univ ≠ univ.erase x := by
+  simp [erase]
 
-theorem diff_erase_self_eq_of_mem {α : Type*} {x : α} {s : Set α}
-(h : x ∈ s) : s \ s.erase x = {x} := by simpa [erase]
+theorem diff_erase_self_eq_of_mem {x : α} (h : x ∈ s) : s \ s.erase x = {x} := by
+  simpa [erase]
 
-theorem eq_empty_iff {α : Type*} {s : Set α} : s = ∅ ↔ ∀ x, x ∉ s :=
+theorem eq_empty_iff : s = ∅ ↔ ∀ x, x ∉ s :=
   eq_empty_iff_forall_notMem
 
 @[simp]
-theorem subsingleton_upair_iff {α : Type*} {x y : α} :
-({x, y} : Set _).Subsingleton ↔ x = y := by
+theorem subsingleton_pair_iff {x y : α} : ({x, y} : Set _).Subsingleton ↔ x = y := by
   simp [Set.Subsingleton]; simp [eq_comm]
 
 @[simp]
-theorem not_nonempty_iff {α : Type*} {s : Set α} :
-¬s.Nonempty ↔ s = ∅ := not_nonempty_iff_eq_empty
+theorem not_nonempty_iff : ¬s.Nonempty ↔ s = ∅ :=
+  not_nonempty_iff_eq_empty
 
 @[simp]
-theorem setOf_compl {α : Type*} {P : α → Prop} :
-{x | P x}ᶜ = {x | ¬P x} := rfl
+theorem setOf_compl {P : α → Prop} : {x | P x}ᶜ = {x | ¬P x} := rfl
 
 @[simp]
-theorem univ_injOn_iff {α β : Type*} {f : α → β} :
-(univ : Set α).InjOn f ↔ f.Injective := by simp [Set.InjOn]; rfl
+theorem univ_injOn_iff {f : α → β} : (univ : Set α).InjOn f ↔ f.Injective := by
+  simp [Set.InjOn]; rfl
+
+@[simp]
+theorem diff_eq_empty' : s \ s' = ∅ ↔ s ⊆ s' := diff_eq_empty
+
+@[simp]
+theorem exists_mem {x} : ∃ (s : Set α), x ∈ s := by
+  use {x}; simp
+
+@[simp]
+theorem iUnion_preimage {f : α → β} : ⋃ b, f ⁻¹' b = univ := by
+  ext x; simp
+
+theorem minimal_le_minimal_of_subset {α : Type*} [ha : LinearOrder α] {s s' : Set α} {x y : α}
+(h₁ : s' ⊆ s) (h₂ : Minimal (· ∈ s') y) (h₃ : Minimal (· ∈ s) x) : x ≤ y := by
+  dsimp [Minimal] at h₂ h₃
+  rcases h₂ with ⟨h₂, h₄⟩
+  rcases h₃ with ⟨h₃, h₅⟩
+  have h₆ := h₁ h₂
+  by_contra! h₇
+  specialize h₅ h₆ (le_of_lt h₇)
+  contrapose! h₇
+  exact h₅
