AP/Util/Nat.lean
@@ -329,3 +329,11 @@ theorem le_exp_right {a b : ℕ} (h : b ≠ 0) : a ≤ a ^ b := by
   cases b; simp at h; rename_i b; simp [pow_add]; cases a
   simp; rename_i a; cases b; simp; rename_i b
   simp [pow_add]; by_contra h₁; simp at h₁
+
+-- #check 0 #exit
+
+theorem find_le_find_of_imp {P Q : ℕ → Prop}
+[hp : DecidablePred P] [hq : DecidablePred Q]
+{h₁ : ∃ n, P n} {h₂ : ∃ n, Q n} (h₃ : ∀ n, Q n → P n) :
+Nat.find h₁ ≤ Nat.find h₂ := by
+  apply Nat.find_le; apply h₃; exact Nat.find_spec h₂
